***NO_CI*** Investigated an intro/elim-form presentation of witnessed, based on the idea of using (witnessed (rel x)) to state that the current state/world is at least (x). But unfortunately, the used intro/elim-rules allow one to prove (p) for all past states of (x).

ulib/FStar.Witnessed.fst
@@ -1,184 +1,215 @@
 module FStar.Witnessed
 
-(* An axiomatisation of the witnessed modality for preorder-indexed state monads *)
+(* Natural deduction for the witnessed modality for preorder-indexed state monads *)
 
 open FStar.Preorder
 
 (* The witnessed modality *)
 
-abstract let witnessed (#s:Type) (#rel:preorder s) (p:predicate s) 
-  = stable p rel //internal representation, guarantees that all assumed witnessed predicates are stable
+assume type witnessed: #s:Type -> rel:preorder s -> p:predicate s -> Type0
 
-(* Every witnessed predicate is stable *)
+(* Syntactic sugar for "current" state/world. *)
 
-val lemma_witnessed_stable: #s:Type
+let is_current_state_wrt (#s:Type) (x:s) (rel:preorder s) = witnessed rel (rel x) 
+
+(* Introduction rule for the witnessed modality*)
+
+assume val witnessed_intro: #s:Type
                          -> #rel:preorder s
+                         -> x:s
                          -> p:predicate s
-                         -> Lemma (requires (witnessed #s #rel p))
-                                  (ensures  (stable p rel))
-let lemma_witnessed_stable #s #rel p = ()
+                         -> Lemma (requires (   x `is_current_state_wrt` rel 
+                                             /\ p x 
+                                             /\ stable p rel))
+                                  (ensures  (witnessed rel p))
+                                  [SMTPat (x `is_current_state_wrt` rel); 
+                                   SMTPat (p x); 
+                                   SMTPat (stable p rel)]
 
-(* The functoriality (introduction) and elimination rules for the witnessed modality *)
+(* Elimination rule for the witnessed modality *)
 
-val ax_fun: #s:Type 
-         -> #rel:preorder s
-         -> p:predicate s{stable p rel} 
-         -> q:predicate s{stable q rel}
-         -> Lemma (requires (forall x . p x ==> q x))
-                  (ensures  (witnessed #s #rel p ==> witnessed #s #rel q))
-let ax_fun #s #rel p q = ()
+assume val witnessed_elim: #s:Type
+                        -> #rel:preorder s
+                        -> x:s
+                        -> x':s
+                        -> p:predicate s
+                        -> Lemma (requires (   x `is_current_state_wrt` rel 
+                                            /\ witnessed rel p 
+                                            /\ rel x x'))
+                                 (ensures  (p x'))
+                                 [SMTPat (witnessed rel (rel x)); 
+                                  SMTPat (witnessed rel p); 
+                                  SMTPat (rel x x')]
 
-(* ax_elim is only valid in a witnessed-free environment *)
+(* 
+   Note that both the intro. and elm. rule are stated relative to the 
+   "current" state/world x. We use the witnessed modality itself to 
+   impose these preconditions. These preconditions will be additionally 
+   assumed WPs of the monotonic state operations. 
+*)
 
-(*val ax_elim: #s:Type
-          -> #rel:preorder s
-          -> p:predicate s
-          -> q:predicate s
-          -> x:s
-          -> Lemma (requires ((witnessed #s #rel p ==> witnessed #s #rel q) /\ p x))
-                   (ensures  (q x))
-let ax_elim #s #rel p q x = admit () //not provable with the current representation of witnessed*)
 
-(* Rules for the interaction of the witnessed modality with other logical connectives *)
+(* All the lemmas below are proved relative to the "current" state/world x. *)
 
-(* These would be part of the deduction system in a dedicated logic for the logic with *)
-(* the witnessed modality. Here they are either proved or assumed as lemmas in F*.     *)
+(* The witnessed modality is functorial. *)
 
-val ax_true: #s:Type
-          -> #rel:preorder s
-          -> Lemma (witnessed #s #rel (fun _ -> True))
-let ax_true #s #rel = ()
-
-val ax_false: #s:Type
-           -> #rel:preorder s
-           -> Lemma (requires (witnessed #s #rel (fun _ -> False)))
-                    (ensures  (False))
-let ax_false #s #rel = admit () //not provable with the current representation of witnessed
-
-val ax_and: #s:Type
-         -> #rel:preorder s
-         -> p:predicate s
-         -> q:predicate s
-         -> Lemma (requires (witnessed #s #rel p /\ witnessed #s #rel q))
-                  (ensures  (witnessed #s #rel (fun x -> p x /\ q x)))
-let ax_and #s #rel p q = ()
-
-val ax_or: #s:Type
-        -> #rel:preorder s
-        -> p:predicate s{stable p rel}
-        -> q:predicate s{stable q rel}
-        -> Lemma (requires (witnessed #s #rel (fun x -> p x \/ q x)))
-                 (ensures  (witnessed #s #rel p \/ witnessed #s #rel q))
-let ax_or #s #rel p q = ()                  
-
-val ax_impl: #s:Type
-          -> #rel:preorder s
-          -> p:predicate s{stable p rel}
-          -> q:predicate s{stable q rel /\ stable (fun x -> p x ==> q x) rel}
-          -> Lemma (requires ((witnessed #s #rel p ==> witnessed #s #rel q)))
-                   (ensures  (witnessed #s #rel (fun x -> p x ==> q x)))
-let ax_impl #s #rel p q = ()
-
-(* Showing that the stability of ax_forall precondition implies the stability of its conclusion *)
-private let lemma_forall_stability_aux (#s:Type) (#rel:preorder s) (p:predicate (s * s))
-  :Lemma (requires ((forall x . stable (fun y -> p (x,y)) rel)))
-         (ensures  (forall y y' . (forall x . p (x,y)) /\ rel y y' ==> (forall x. p (x,y'))))
+let witnessed_functoriality (#s:Type) (#rel:preorder s) (x:s) (p:predicate s) (q:predicate s)
+  : Lemma (requires (   x `is_current_state_wrt` rel
+                     /\ (forall y . p y ==> q y)
+                     /\ stable p rel
+                     /\ stable q rel))
+          (ensures  (witnessed rel p ==> witnessed rel q))
   = ()
 
-private let lemma_forall_stability (#s:Type) (#rel:preorder s) (p:predicate (s * s))
-  :Lemma (requires (forall x . stable (fun y -> p (x,y)) rel)) 
-         (ensures  (stable (fun y -> (forall x . p (x,y))) rel))
-  = lemma_forall_stability_aux #s #rel p
+(* Showing how witnessed interacts with other logical connectives. *)
 
-val ax_forall: #s:Type
-            -> #rel:preorder s
-            -> p:predicate (s * s)
-            -> Lemma (requires (forall x . witnessed #s #rel (fun y -> p (x,y))))
-                     (ensures  (witnessed #s #rel (fun y -> forall x . p (x,y))))
-let ax_forall #s #rel p = admit () //not provable with the current representation of witnessed
+let witnessed_true (#s:Type) (#rel:preorder s) (x:s) (p:predicate s)
+  : Lemma (requires (x `is_current_state_wrt` rel))
+          (ensures  (witnessed rel (fun _ -> True)))
+  = witnessed_intro #s #rel x (fun _ -> True)
 
-val ax_exists: #s:Type
-            -> #rel:preorder s
-            -> p:predicate (s * s){forall y . stable (fun x -> p (x,y)) rel} //analogous assumption to ax_or
-            -> Lemma (requires (witnessed #s #rel (fun x -> exists y . p (x,y))))
-                     (ensures  (exists y . witnessed #s #rel (fun x -> p (x,y))))
-let ax_exists #s #rel p = admit () //not provable with the current representation of witnessed
-
-(* Using the axioms above, the witnessed modality in fact commutes with other logical connectives *)
-
-val lemma_true: #s:Type
-             -> #rel:preorder s
-             -> Lemma (witnessed #s #rel (fun _ -> True) 
-                       <==> 
-                       True)
-let lemma_true #s #rel = ()
-
-val lemma_false: #s:Type
-              -> #rel:preorder s
-              -> Lemma (witnessed #s #rel (fun _ -> False) 
-                        <==> 
-                        False)
-let lemma_false #s #rel = ax_false #s #rel
-
-val lemma_and: #s:Type
-            -> #rel:preorder s
-            -> p:predicate s
-            -> q:predicate s
-            -> Lemma (requires (stable p rel /\ stable q rel))
-                     (ensures  ((witnessed #s #rel p /\ witnessed #s #rel q) 
-                                <==> 
-                                (witnessed #s #rel (fun x -> p x /\ q x))))
-let lemma_and #s #rel p q = ()
-
-val lemma_or: #s:Type
-           -> #rel:preorder s
-           -> p:predicate s
-           -> q:predicate s
-           -> Lemma (requires (stable p rel /\ stable q rel))
-                    (ensures  ((witnessed #s #rel (fun x -> p x \/ q x)) 
-                               <==> 
-                               (witnessed #s #rel p \/ witnessed #s #rel q)))
-let lemma_or #s #rel p q = ()                  
-
-val lemma_impl: #s:Type
-             -> #rel:preorder s
-             -> p:predicate s
-             -> q:predicate s
-             -> Lemma (requires (stable p rel /\ stable q rel /\ stable (fun x -> p x ==> q x) rel))
-                      (ensures  (((witnessed #s #rel p ==> witnessed #s #rel q)) 
-                                 <==> 
-                                 (witnessed #s #rel (fun x -> p x ==> q x))))
-let lemma_impl #s #rel p q = ()
-
-val lemma_forall: #s:Type
-               -> #rel:preorder s
-               -> p:predicate (s * s)
-               -> Lemma (requires (forall x . stable (fun y -> p (x,y)) rel))
-                        (ensures  ((forall x . witnessed #s #rel (fun y -> p (x,y))) 
-                                   <==> 
-                                   (witnessed #s #rel (fun y -> forall x . p (x,y)))))
-let lemma_forall #s #rel p = ax_forall #s #rel p
-
-let lemma_exists_aux (#s:Type) (#rel:preorder s) (p:predicate (s * s))
-  :Lemma (requires (forall y . stable (fun x -> p (x,y)) rel))
-         (ensures  (forall x x' . (exists y . p(x,y)) /\ rel x x' ==> (exists y . p (x',y))))
+let witnessed_false (#s:Type) (#rel:preorder s) (x:s) (p:predicate s)
+  : Lemma (requires (   x `is_current_state_wrt` rel 
+                     /\ witnessed rel (fun _ -> False)))
+          (ensures  (False))
   = ()
 
-val lemma_exists: #s:Type
-               -> #rel:preorder s
-               -> p:predicate (s * s)
-               -> Lemma (requires ((forall y . stable (fun x -> p (x,y)) rel)))
-                        (ensures  ((witnessed #s #rel (fun x -> exists y . p (x,y))) 
-                                   <==> 
-                                   (exists y . (witnessed #s #rel (fun x -> p (x,y))))))
-let lemma_exists #s #rel p = lemma_exists_aux #s #rel p; ax_exists #s #rel p
+let witnessed_and1 (#s:Type) (#rel:preorder s) (x:s) (p:predicate s) (q:predicate s)
+  : Lemma (requires (   x `is_current_state_wrt` rel
+                     /\ witnessed rel p
+                     /\ witnessed rel q
+                     /\ stable p rel
+                     /\ stable q rel))
+          (ensures  (witnessed rel (fun y -> p y /\ q y)))
+  = witnessed_intro #s #rel x (fun y -> p y /\ q y)
 
-(* A useful lemma for the metatheory, allows us to introduce witnessed relative to the "current" world *)
+let witnessed_and2 (#s:Type) (#rel:preorder s) (x:s) (p:predicate s) (q:predicate s)
+  : Lemma (requires (   x `is_current_state_wrt` rel
+                     /\ witnessed rel (fun y -> p y /\ q y)
+                     /\ stable p rel
+                     /\ stable q rel))
+          (ensures  (witnessed rel p /\ witnessed rel q))
+  = ()
 
-val lemma_relative_intro: #s:Type
-                       -> #rel:preorder s
-                       -> p:predicate s
-                       -> x:s
-                       -> Lemma (requires ((witnessed #s #rel (fun y -> rel x y) ==> p x) /\ stable p rel))
-                                (ensures  (witnessed #s #rel (fun y -> rel x y) ==> witnessed #s #rel p))
-let lemma_relative_intro #s #rel p x = ()
+let witnessed_or1 (#s:Type) (#rel:preorder s) (x:s) (p:predicate s) (q:predicate s)
+  : Lemma (requires (   x `is_current_state_wrt` rel
+                     /\ witnessed rel (fun y -> p x \/ q x)
+                     /\ stable p rel
+                     /\ stable q rel))
+          (ensures  (witnessed rel p \/ witnessed rel q))
+  = ()
+
+let witnessed_or2 (#s:Type) (#rel:preorder s) (x:s) (p:predicate s) (q:predicate s)
+  : Lemma (requires (   x `is_current_state_wrt` rel
+                     /\ (witnessed rel p \/ witnessed rel q)
+                     /\ stable p rel
+                     /\ stable q rel))
+          (ensures  (witnessed rel (fun y -> p y \/ q y)))
+  = witnessed_intro #s #rel x (fun y -> p y \/ q y)
+
+let witnessed_forall1 (#s:Type) (#rel:preorder s) (x:s) (p:predicate (s * s))
+  : Lemma (requires (   x `is_current_state_wrt` rel
+                     /\ (forall y . witnessed rel (fun z -> p (y,z)))
+                     /\ stable (fun z -> forall y . p (y,z)) rel))
+          (ensures  (witnessed rel (fun z -> forall y . p (y,z))))
+  = witnessed_intro #s #rel x (fun z -> forall y . p (y,z))
+
+let witnessed_forall2_aux (#s:Type) (#rel:preorder s) (x:s) (p:predicate (s * s)) (y:s)
+  : Lemma (requires (   x `is_current_state_wrt` rel
+                     /\ witnessed rel (fun z -> forall y . p (y,z))
+                     /\ (forall y . stable (fun z -> p (y,z)) rel)))
+          (ensures  (witnessed rel (fun z -> p (y,z))))
+          [SMTPat (x `is_current_state_wrt` rel);
+           SMTPat (witnessed rel (fun z -> forall y . p (y,z))); 
+           SMTPat (stable (fun z -> p (y,z)) rel)]
+  = witnessed_intro #s #rel x (fun z -> p (y,z))
+
+let witnessed_forall2 (#s:Type) (#rel:preorder s) (x:s) (p:predicate (s * s))
+  : Lemma (requires (   x `is_current_state_wrt` rel
+                     /\ witnessed rel (fun z -> forall y . p (y,z))
+                     /\ (forall y . stable (fun z -> p (y,z)) rel)))
+          (ensures  (forall y . witnessed rel (fun z -> p (y,z))))
+  = ()
+
+let witnessed_exists1_aux (#s:Type) (#rel:preorder s) (x:s) (p:predicate (s * s)) (y:s)
+  : Lemma (requires (   x `is_current_state_wrt` rel
+                     /\ p (y,x)
+                     /\ (forall y . stable (fun z -> p (y,z)) rel)))
+          (ensures  (ensures  (exists y . witnessed rel (fun z -> p (y,z)))))
+          [SMTPat (x `is_current_state_wrt` rel);
+           SMTPat (stable (fun z -> p (y,z)) rel)]
+  = witnessed_intro #s #rel x (fun z -> p (y,z))
+
+let witnessed_exists1 (#s:Type) (#rel:preorder s) (x:s) (p:predicate (s * s))
+  : Lemma (requires (   x `is_current_state_wrt` rel
+                     /\ witnessed rel (fun z -> exists y . p (y,z))
+                     /\ (forall y . stable (fun z -> p (y,z)) rel)))
+          (ensures  (exists y . witnessed rel (fun z -> p (y,z))))
+  = witnessed_elim #s #rel x x (fun z -> exists y . p (y,z))
+
+let witnessed_exists2 (#s:Type) (#rel:preorder s) (x:s) (p:predicate (s * s))
+  : Lemma (requires (   x `is_current_state_wrt` rel
+                     /\ (exists y . witnessed rel (fun z -> p (y,z)))
+                     /\ (stable (fun z -> exists y . p (y,z)) rel)))
+          (ensures  (witnessed rel (fun z -> exists y . p (y,z))))
+  = witnessed_intro #s #rel x (fun z -> exists y . p (y,z))
+
+let witnessed_impl1 (#s:Type) (#rel:preorder s) (x:s) (p:predicate s) (q:predicate s)
+  : Lemma (requires (   x `is_current_state_wrt` rel
+                     /\ witnessed rel (fun y -> p y ==> q y)
+                     /\ stable p rel
+                     /\ stable q rel))
+          (ensures  (witnessed rel p ==> witnessed rel q))
+  = ()
+
+let witnessed_impl2_aux1 (#s:Type) (#rel:preorder s) (x:s) (p:predicate s) (q:predicate s)
+  : Lemma (requires (   x `is_current_state_wrt` rel
+                     /\ (forall y . (p y /\ rel y x) ==> q y)
+                     /\ stable p rel
+                     /\ stable q rel
+                     /\ stable (fun y -> (p y /\ rel y x) ==> q y) rel))
+          (ensures  (witnessed rel (fun y -> (p y /\ rel y x) ==> q y)))
+  = witnessed_intro #s #rel x (fun y -> (p y /\ rel y x) ==> q y)
+
+let witnessed_impl2_aux2 (#s:Type) (#rel:preorder s) (x:s) (p:predicate s) (q:predicate s) (y:s)
+  : Lemma (requires (   x `is_current_state_wrt` rel
+                     /\ (witnessed rel p ==> witnessed rel q)
+                     /\ stable p rel
+                     /\ stable q rel
+                     /\ p y
+                     /\ rel y x))
+          (ensures  (q y))
+          [SMTPat (x `is_current_state_wrt` rel);
+           SMTPat (witnessed rel p ==> witnessed rel q);
+           SMTPat (p y);
+           SMTPat (rel y x)]
+  = witnessed_intro #s #rel x (rel y);
+    witnessed_intro #s #rel y p;
+    witnessed_elim #s #rel y y q
+
+let witnessed_impl2 (#s:Type) (#rel:preorder s) (x:s) (p:predicate s) (q:predicate s)
+  : Lemma (requires (   x `is_current_state_wrt` rel
+                     /\ (witnessed rel p ==> witnessed rel q)
+                     /\ stable p rel
+                     /\ stable q rel
+                     /\ stable (fun y -> (p y /\ rel y x) ==> q y) rel))
+          (ensures  (witnessed rel (fun y -> (p y /\ rel y x) ==> q y)))
+  = assert (witnessed rel p ==> witnessed rel q); //used to trigger witnessed_impl2_aux2
+    witnessed_impl2_aux1 #s #rel x p q
+
+
+(* 
+   A lemma showing a suspicious behaviour of this exiomatisation of witnessed.
+
+   When we use (witnessed rel (rel x)) to make an assumption that x is our "current" 
+   state/world, then we can prove the predicate p for all past worlds of x, which 
+   surely should not be the case!?! 
+*)
+
+let suspicious_lemma (#s:Type) (#rel:preorder s) (x:s) (p:predicate s) (q:predicate s) (y:s)
+  : Lemma (requires (   x `is_current_state_wrt` rel
+                     /\ witnessed rel p
+                     /\ stable p rel
+                     /\ rel y x))
+          (ensures  (p y))
+  = witnessed_intro #s #rel x (rel y)
